src/Ex/SingleValue.v
@@ -24,78 +24,97 @@ Definition svmGetIdx: IdxT := 0.
 Definition svmSetIdx: IdxT := 1.
 
 Section System.
-  Variables erq1 erq2 ers1 ers2: nat.
 
-  Definition c1pRq := 0.
-  Definition c1pRs := 1.
-  Definition pc1 := 2.
-  Definition c2pRq := 3.
-  Definition c2pRs := 4.
-  Definition pc2 := 5.
-  
-  Hypothesis (Hmvalid: NoDup ([c1pRq; c1pRs; pc1; c2pRq; c2pRs; pc2]
-                                ++ [erq1; erq2; ers1; ers2])).
+  Definition erq1 := 0.
+  Definition ers1 := 1.
+  Definition c1pRq := 2.
+  Definition c1pRs := 3.
+  Definition pc1 := 4.
+
+  Definition erq2 := 5.
+  Definition ers2 := 6.
+  Definition c2pRq := 7.
+  Definition c2pRs := 8.
+  Definition pc2 := 9.
+
+  Definition svm_msg_inds_valid:
+    NoDup ([c1pRq; c1pRs; pc1; c2pRq; c2pRs; pc2]
+             ++ [erq1; erq2; ers1; ers2]).
+  Proof.
+    compute; repeat (constructor; firstorder).
+  Qed.
 
   Section Spec.
 
     Definition specIdx := 0.
     Definition valueIdx := 0.
+
+    Definition SpecOStateIfc: OStateIfc :=
+      {| ost_sz := 1;
+         ost_ty :=
+           fun n =>
+             match n with
+             | O => nat
+             | _ => unit
+             end
+      |}.
     
     Section PerChn.
       Variables erq ers: nat.
 
-      Definition specGetRq: Rule :=
-        {| rule_oidx := specIdx;
+      Definition specGetRq: Rule SpecOStateIfc :=
+        {| rule_idx := 0; (* TODO: fix it, it's wrong. *)
            rule_msg_ids := svmGetIdx :: nil;
            rule_minds := erq :: nil;
            rule_precond := ⊤oprec;
            rule_trs :=
-             fun ost orq mins =>
+             fun (ost: OState SpecOStateIfc) orq mins =>
                (ost, orq,
-                ost@[valueIdx] >>=[nil]
-                   (fun v => (ers, {| msg_id := svmGetIdx;
-                                      msg_rr := Rq;
-                                      msg_value := v |})
-                               :: nil))
+                (ers, {| msg_id := svmGetIdx;
+                         msg_rr := Rq;
+                         msg_value := VNat (IList.ith ost Fin.F1) |}) :: nil)
         |}.
 
-      Definition specSetRq: Rule :=
-        {| rule_oidx := specIdx;
-           rule_msg_ids := svmSetIdx :: nil;
-           rule_minds := erq :: nil;
-           rule_precond := ⊤oprec;
-           rule_trs :=
-             fun ost orq mins =>
-               ((hd_error mins) >>=[ost]
-                (fun idm => ost+[valueIdx <- msg_value (valOf idm)]),
-                orq,
-                ((ers, {| msg_id := svmSetIdx;
-                          msg_rr := Rq;
-                          msg_value := VUnit |})
-                   :: nil))
-        |}.
+      (* Definition specSetRq: Rule := *)
+      (*   {| rule_oidx := specIdx; *)
+      (*      rule_msg_ids := svmSetIdx :: nil; *)
+      (*      rule_minds := erq :: nil; *)
+      (*      rule_precond := ⊤oprec; *)
+      (*      rule_trs := *)
+      (*        fun ost orq mins => *)
+      (*          ((hd_error mins) >>=[ost] *)
+      (*           (fun idm => ost+[valueIdx <- msg_value (valOf idm)]), *)
+      (*           orq, *)
+      (*           ((ers, {| msg_id := svmSetIdx; *)
+      (*                     msg_rr := Rq; *)
+      (*                     msg_value := VUnit |}) *)
+      (*              :: nil)) *)
+      (*   |}. *)
 
     End PerChn.
 
-    Definition specInit: OStates := [specIdx <- [valueIdx <- VNat 0]].
+    (* Definition specInit: OStates := *)
+    (*   [specIdx <- {| ost_ifc := SpecOStateIfc; *)
+    (*                  ost_st := {| IList.prim_fst := 0; *)
+    (*                               IList.prim_snd := tt |} |}]. *)
 
-    Definition spec: System :=
-      {| sys_oinds := specIdx :: nil;
-         sys_minds := nil;
-         sys_merqs := erq1 :: erq2 :: nil;
-         sys_merss := ers1 :: ers2 :: nil;
-         sys_msg_inds_valid := NoDup_app_weakening_2 _ _ Hmvalid;
-         sys_inits := specInit;
-         sys_rules :=
-           (specGetRq erq1 ers1)
-             :: (specSetRq erq1 ers1)
-             :: (specGetRq erq2 ers2)
-             :: (specSetRq erq2 ers2) :: nil
-      |}.
+    (* Definition spec: System := *)
+    (*   {| sys_oinds := specIdx :: nil; *)
+    (*      sys_minds := nil; *)
+    (*      sys_merqs := erq1 :: erq2 :: nil; *)
+    (*      sys_merss := ers1 :: ers2 :: nil; *)
+    (*      sys_msg_inds_valid := NoDup_app_weakening_2 _ _ Hmvalid; *)
+    (*      sys_inits := specInit; *)
+    (*      sys_rules := *)
+    (*        (specGetRq erq1 ers1) *)
+    (*          :: (specSetRq erq1 ers1) *)
+    (*          :: (specGetRq erq2 ers2) *)
+    (*          :: (specSetRq erq2 ers2) :: nil *)
+    (*   |}. *)
 
   End Spec.
 
-  Section Impl0.
+  Section Impl.
 
     Definition parentIdx := 0.
     Definition child1Idx := 1.
@@ -108,35 +127,67 @@ Section System.
     Definition stS := 1.
     Definition stI := 0.
 
-    Definition implInit: OStates :=
-      [parentIdx <- [valueIdx <- VNat 0] +[statusIdx <- VNat stS]]
-      +[child1Idx <- [valueIdx <- VNat 0] +[statusIdx <- VNat stS]]
-      +[child2Idx <- [valueIdx <- VNat 0] +[statusIdx <- VNat stS]].
+    (* Definition implInit: OStates := *)
+    (*   [parentIdx <- [valueIdx <- VNat 0] +[statusIdx <- VNat stS]] *)
+    (*   +[child1Idx <- [valueIdx <- VNat 0] +[statusIdx <- VNat stS]] *)
+    (*   +[child2Idx <- [valueIdx <- VNat 0] +[statusIdx <- VNat stS]]. *)
 
-    Definition impl0: System :=
-      {| sys_oinds := parentIdx :: child1Idx :: child2Idx :: nil;
-         sys_minds := c1pRq :: c1pRs :: pc1 :: c2pRq :: c2pRs :: pc2 :: nil;
-         sys_merqs := erq1 :: erq2 :: nil;
-         sys_merss := ers1 :: ers2 :: nil;
-         sys_msg_inds_valid := Hmvalid;
-         sys_inits := implInit;
-         sys_rules := nil |}.
+    Section PerChild.
+      Variables (erq ers: nat) (oidx: IdxT).
 
-    Definition implTopo: GTree :=
-      Node parentIdx
-           [([createEdge child1Idx c1pRq parentIdx;
-                createEdge child1Idx c1pRs parentIdx;
-                createEdge parentIdx pc1 child1Idx],
-             Node child1Idx nil);
-              ([createEdge child2Idx parentIdx c2pRq;
-                  createEdge child2Idx parentIdx c2pRs;
-                  createEdge parentIdx child2Idx pc2],
-               Node child2Idx nil)].
-                                            
-    Definition implIndices: list IdxT :=
-      ltac:(evalOIndsOf impl0).
+      (* Definition implGetImm: Rule := *)
+      (*   {| rule_oidx := oidx; *)
+      (*      rule_msg_ids := svmGetIdx :: nil; *)
+      (*      rule_minds := erq :: nil; *)
+      (*      rule_precond := *)
+      (*        fun ost orq mins => *)
+      (*          ost@[statusIdx] >=[False] (fun st => st >= stS); *)
+      (*      rule_trs := *)
+      (*        fun ost orq mins => *)
+      (*          (ost, orq, *)
     
-  End Impl0.
+      (* Definition implGetRqUp: Rule := *)
+      (*   {| rule_oidx := oidx; *)
+      (*      rule_msg_ids := svmGetIdx :: nil; *)
+      (*      rule_minds := erq :: nil; *)
+      (*      rule_precond := *)
+      (*        fun ost orq mins => True; *)
+      (*      rule_trs := *)
+      (*        fun ost orq mins => *)
+      (*          (ost, orq, *)
+      (*           ost@[valueIdx] >>=[nil] *)
+      (*              (fun v => (ers, {| msg_id := svmGetIdx; *)
+      (*                                 msg_rr := Rq; *)
+      (*                                 msg_value := v |}) *)
+      (*                          :: nil)) *)
+      (*   |}. *)
+
+    End PerChild.
+    
+    (* Definition impl0: System := *)
+    (*   {| sys_oinds := parentIdx :: child1Idx :: child2Idx :: nil; *)
+    (*      sys_minds := c1pRq :: c1pRs :: pc1 :: c2pRq :: c2pRs :: pc2 :: nil; *)
+    (*      sys_merqs := erq1 :: erq2 :: nil; *)
+    (*      sys_merss := ers1 :: ers2 :: nil; *)
+    (*      sys_msg_inds_valid := Hmvalid; *)
+    (*      sys_inits := implInit; *)
+    (*      sys_rules := nil |}. *)
+
+    (* Definition implTopo: GTree := *)
+    (*   Node parentIdx *)
+    (*        [([createEdge child1Idx c1pRq parentIdx; *)
+    (*             createEdge child1Idx c1pRs parentIdx; *)
+    (*             createEdge parentIdx pc1 child1Idx], *)
+    (*          Node child1Idx nil); *)
+    (*           ([createEdge child2Idx parentIdx c2pRq; *)
+    (*               createEdge child2Idx parentIdx c2pRs; *)
+    (*               createEdge parentIdx child2Idx pc2], *)
+    (*            Node child2Idx nil)]. *)
+                                            
+    (* Definition implIndices: list IdxT := *)
+    (*   ltac:(evalOIndsOf impl0). *)
+    
+  End Impl.
 
 End System.
 
