src/Ex/SingleValueSim.v
@@ -1,7 +1,7 @@
 Require Import Bool List String Peano_dec.
 Require Import Common FMap Syntax Topology Semantics SemFacts StepM StepT.
-Require Import Invariant Simulation TrsSim SerialFacts.
-Require Import PredMsg Blocking.
+Require Import Invariant Simulation SerialFacts.
+Require Import Blocking.
 
 Require Import SingleValue.
 
@@ -10,170 +10,172 @@ Set Implicit Arguments.
 Open Scope list.
 Open Scope fmap.
 
-Section OPrecs.
+(** * TODO: recover all below with new notations. *)
 
-  Definition ImplOStatusM: OPrec :=
-    fun ost _ _ => ost@[statusIdx] = Some (VNat stM).
+(* Section OPrecs. *)
 
-  Definition ImplOStatusS: OPrec :=
-    fun ost _ _ => ost@[statusIdx] = Some (VNat stS).
+(*   Definition ImplOStatusM: OPrec := *)
+(*     fun ost _ _ => ost@[statusIdx] = Some (VNat stM). *)
+
+(*   Definition ImplOStatusS: OPrec := *)
+(*     fun ost _ _ => ost@[statusIdx] = Some (VNat stS). *)
   
-  Definition ImplOStatusI: OPrec :=
-    fun ost _ _ => ost@[statusIdx] = Some (VNat stI).
+(*   Definition ImplOStatusI: OPrec := *)
+(*     fun ost _ _ => ost@[statusIdx] = Some (VNat stI). *)
 
-End OPrecs.
+(* End OPrecs. *)
 
-Section Predicates.
+(* Section Predicates. *)
 
-  Definition ImplStateI: OStatesFP :=
-    OStateForallP
-      (fun oidx ost =>
-         forall stt, 
-           ost@[statusIdx] = Some (VNat stt) ->
-           stt = stI).
+(*   Definition ImplStateI: OStatesFP := *)
+(*     OStateForallP *)
+(*       (fun oidx ost => *)
+(*          forall stt,  *)
+(*            ost@[statusIdx] = Some (VNat stt) -> *)
+(*            stt = stI). *)
 
-  Definition ImplStateMI (v: Value): OStatesFP :=
-    fun inds ioss =>
-      exists midx,
-        In midx inds /\
-        OStateExistsP
-          (fun oidx ost =>
-             ost@[statusIdx] = Some (VNat stM) /\
-             ost@[valueIdx] = Some v) midx ioss /\
-        OStateForallP
-          (fun oidx ost =>
-             oidx <> midx ->
-             forall stt,
-               ost@[statusIdx] = Some (VNat stt) ->
-               stt = stI) inds ioss.
+(*   Definition ImplStateMI (v: Value): OStatesFP := *)
+(*     fun inds ioss => *)
+(*       exists midx, *)
+(*         In midx inds /\ *)
+(*         OStateExistsP *)
+(*           (fun oidx ost => *)
+(*              ost@[statusIdx] = Some (VNat stM) /\ *)
+(*              ost@[valueIdx] = Some v) midx ioss /\ *)
+(*         OStateForallP *)
+(*           (fun oidx ost => *)
+(*              oidx <> midx -> *)
+(*              forall stt, *)
+(*                ost@[statusIdx] = Some (VNat stt) -> *)
+(*                stt = stI) inds ioss. *)
 
-  Definition ImplStateSI (v: Value): OStatesFP :=
-    fun inds ioss =>
-      (exists midx,
-          In midx inds /\
-          OStateExistsP
-            (fun oidx ost => ost@[statusIdx] = Some (VNat stS)) midx ioss) /\
-      OStateForallP
-        (fun oidx ost =>
-           forall stt,
-             ost@[statusIdx] = Some (VNat stt) ->
-             match stt with
-             | 0 (* stI *) => True
-             | 1 (* stS *) => ost@[valueIdx] = Some v
-             | 2 (* stM *) => False
-             | _ => False
-             end) inds ioss.
+(*   Definition ImplStateSI (v: Value): OStatesFP := *)
+(*     fun inds ioss => *)
+(*       (exists midx, *)
+(*           In midx inds /\ *)
+(*           OStateExistsP *)
+(*             (fun oidx ost => ost@[statusIdx] = Some (VNat stS)) midx ioss) /\ *)
+(*       OStateForallP *)
+(*         (fun oidx ost => *)
+(*            forall stt, *)
+(*              ost@[statusIdx] = Some (VNat stt) -> *)
+(*              match stt with *)
+(*              | 0 (* stI *) => True *)
+(*              | 1 (* stS *) => ost@[valueIdx] = Some v *)
+(*              | 2 (* stM *) => False *)
+(*              | _ => False *)
+(*              end) inds ioss. *)
 
-  Definition ImplStateMSI (v: Value): OStatesFP :=
-    fun inds ioss => ImplStateMI v inds ioss \/ ImplStateSI v inds ioss.
+(*   Definition ImplStateMSI (v: Value): OStatesFP := *)
+(*     fun inds ioss => ImplStateMI v inds ioss \/ ImplStateSI v inds ioss. *)
 
-  (* NOTE: Here indeed binary predicates are required; if the predicate only
-   * takes a poststate, then we cannot specify that the coherence value should
-   * not be changed.
-   *)
-  (** --(.)--> [MSI(v) -> MSI(v)] --(v)--> *)
-  Definition PredGet (tinds: list IdxT): PredOS :=
-    fun _ poss outv noss =>
-      ImplStateMSI outv tinds poss /\ ImplStateMSI outv tinds noss.
+(*   (* NOTE: Here indeed binary predicates are required; if the predicate only *)
+(*    * takes a poststate, then we cannot specify that the coherence value should *)
+(*    * not be changed. *)
+(*    *) *)
+(*   (** --(.)--> [MSI(v) -> MSI(v)] --(v)--> *) *)
+(*   Definition PredGet (tinds: list IdxT): PredOS := *)
+(*     fun _ poss outv noss => *)
+(*       ImplStateMSI outv tinds poss /\ ImplStateMSI outv tinds noss. *)
 
-  (** --(v)--> [. -> MSI(v)] --(.)--> *)
-  Definition PredSet (tinds: list IdxT): PredOS :=
-    fun inv _ _ noss => ImplStateMI inv tinds noss.
+(*   (** --(v)--> [. -> MSI(v)] --(.)--> *) *)
+(*   Definition PredSet (tinds: list IdxT): PredOS := *)
+(*     fun inv _ _ noss => ImplStateMI inv tinds noss. *)
 
-  (** --(.)--> [MSI(v)|{tinds} -> SI(v)|{tinds}] --(v)--> *)
-  Definition PredGetSI (tinds: list IdxT): PredOS :=
-    fun _ poss outv noss =>
-      ImplStateMSI outv tinds poss /\
-      ImplStateSI outv tinds noss.
+(*   (** --(.)--> [MSI(v)|{tinds} -> SI(v)|{tinds}] --(v)--> *) *)
+(*   Definition PredGetSI (tinds: list IdxT): PredOS := *)
+(*     fun _ poss outv noss => *)
+(*       ImplStateMSI outv tinds poss /\ *)
+(*       ImplStateSI outv tinds noss. *)
 
-  (** --(.)--> [. -> I|{tinds}] --(v)--> *)
-  Definition PredSetI (tinds: list IdxT): PredOS :=
-    fun _ _ _ noss =>
-      ImplStateI tinds noss.
+(*   (** --(.)--> [. -> I|{tinds}] --(v)--> *) *)
+(*   Definition PredSetI (tinds: list IdxT): PredOS := *)
+(*     fun _ _ _ noss => *)
+(*       ImplStateI tinds noss. *)
 
-  Definition OPredGetS: OPred :=
-    fun inv post outv nost =>
-      nost@[statusIdx] = Some (VNat stS) /\
-      nost@[valueIdx] = Some outv.
+(*   Definition OPredGetS: OPred := *)
+(*     fun inv post outv nost => *)
+(*       nost@[statusIdx] = Some (VNat stS) /\ *)
+(*       nost@[valueIdx] = Some outv. *)
 
-  (* Definition getRqFwdF (topo: Tree unit) (rqpmid: PMsgId TMsg): list (PMsgId TMsg) := *)
-  (*   let from := mid_from (pmid_mid rqpmid) in *)
-  (*   let this := mid_to (pmid_mid rqpmid) in *)
-  (*   map (fun tofwds => *)
-  (*          {| pmid_mid := *)
-  (*               {| mid_addr := *)
-  (*                    {| ma_from := this; *)
-  (*                       ma_to := fst tofwds; *)
-  (*                       ma_chn := rqChn |}; *)
-  (*                  mid_tid := mid_tid (pmid_mid rqpmid) |}; *)
-  (*             pmid_pred := *)
-  (*               {| pred_os := PredGetSI (snd tofwds); *)
-  (*                  pred_mp := ⊤ |} *)
-  (*          |}) *)
-  (*       (getFwds topo from this). *)
+(*   (* Definition getRqFwdF (topo: Tree unit) (rqpmid: PMsgId TMsg): list (PMsgId TMsg) := *) *)
+(*   (*   let from := mid_from (pmid_mid rqpmid) in *) *)
+(*   (*   let this := mid_to (pmid_mid rqpmid) in *) *)
+(*   (*   map (fun tofwds => *) *)
+(*   (*          {| pmid_mid := *) *)
+(*   (*               {| mid_addr := *) *)
+(*   (*                    {| ma_from := this; *) *)
+(*   (*                       ma_to := fst tofwds; *) *)
+(*   (*                       ma_chn := rqChn |}; *) *)
+(*   (*                  mid_tid := mid_tid (pmid_mid rqpmid) |}; *) *)
+(*   (*             pmid_pred := *) *)
+(*   (*               {| pred_os := PredGetSI (snd tofwds); *) *)
+(*   (*                  pred_mp := ⊤ |} *) *)
+(*   (*          |}) *) *)
+(*   (*       (getFwds topo from this). *) *)
   
-End Predicates.
+(* End Predicates. *)
 
-Section Sim.
-  Variables erq1 erq2 ers1 ers2: nat.
-  Hypothesis (Hmvalid: NoDup ([c1pRq; c1pRs; pc1; c2pRq; c2pRs; pc2]
-                                ++ [erq1; erq2; ers1; ers2])).
+(* Section Sim. *)
+(*   Variables erq1 erq2 ers1 ers2: nat. *)
+(*   Hypothesis (Hmvalid: NoDup ([c1pRq; c1pRs; pc1; c2pRq; c2pRs; pc2] *)
+(*                                 ++ [erq1; erq2; ers1; ers2])). *)
 
-  Local Notation spec := (spec Hmvalid).
-  Local Notation impl0 := (impl0 Hmvalid).
+(*   Local Notation spec := (spec Hmvalid). *)
+(*   Local Notation impl0 := (impl0 Hmvalid). *)
 
-  (** Global invariants *)
+(*   (** Global invariants *) *)
 
-  Definition SvmInvs :=
-    ValidTrss impl0 /\i BlockedInv /\i ValidTidState.
+(*   Definition SvmInvs := *)
+(*     ValidTrss impl0 /\i BlockedInv /\i ValidTidState. *)
 
-  (** Simulation between [TState]s *)
+(*   (** Simulation between [TState]s *) *)
 
-  Definition SvmSpecState (v: Value) (soss: OStates) :=
-    exists sost,
-      soss@[specIdx] = Some sost /\
-      sost@[valueIdx] = Some v.
+(*   Definition SvmSpecState (v: Value) (soss: OStates) := *)
+(*     exists sost, *)
+(*       soss@[specIdx] = Some sost /\ *)
+(*       sost@[valueIdx] = Some v. *)
 
-  Definition SvmR (tinds: list IdxT): OStates -> OStates -> Prop :=
-    fun ioss soss =>
-      exists cv,
-        ImplStateMSI cv tinds ioss /\ SvmSpecState cv soss.
+(*   Definition SvmR (tinds: list IdxT): OStates -> OStates -> Prop := *)
+(*     fun ioss soss => *)
+(*       exists cv, *)
+(*         ImplStateMSI cv tinds ioss /\ SvmSpecState cv soss. *)
 
-  Definition SvmSpecORqs (sorqs: ORqs TMsg) :=
-    exists sorq,
-      sorqs@[specIdx] = Some sorq.
+(*   Definition SvmSpecORqs (sorqs: ORqs TMsg) := *)
+(*     exists sorq, *)
+(*       sorqs@[specIdx] = Some sorq. *)
 
-  Definition SvmSim {SysT} `{IsSystem SysT} (impl: SysT): TState -> TState -> Prop :=
-    fun ist sst =>
-      SvmR (oindsOf impl) (tst_oss ist) (tst_oss sst) /\
-      SvmSpecORqs (tst_orqs sst) /\
-      SimMP ist sst.
+(*   Definition SvmSim {SysT} `{IsSystem SysT} (impl: SysT): TState -> TState -> Prop := *)
+(*     fun ist sst => *)
+(*       SvmR (oindsOf impl) (tst_oss ist) (tst_oss sst) /\ *)
+(*       SvmSpecORqs (tst_orqs sst) /\ *)
+(*       SimMP ist sst. *)
 
-  Section Facts.
+(*   Section Facts. *)
 
-    Lemma SvmSim_init:
-      SvmSim impl0 (initsOf impl0) (initsOf spec).
-    Proof.
-      repeat esplit.
-      right; repeat econstructor;
-        cbn; intros; inv H; cbn; reflexivity.
-    Qed.
+(*     Lemma SvmSim_init: *)
+(*       SvmSim impl0 (initsOf impl0) (initsOf spec). *)
+(*     Proof. *)
+(*       repeat esplit. *)
+(*       right; repeat econstructor; *)
+(*         cbn; intros; inv H; cbn; reflexivity. *)
+(*     Qed. *)
 
-    Lemma SvmSim_MsgsSim:
-      MsgsSim (SvmSim impl0).
-    Proof.
-    Admitted.
+(*     Lemma SvmSim_MsgsSim: *)
+(*       MsgsSim (SvmSim impl0). *)
+(*     Proof. *)
+(*     Admitted. *)
 
-    Lemma SvmInvs_init:
-      SvmInvs (initsOf impl0).
-    Proof.
-      repeat constructor.
-      - hnf; intros.
-        elim H.
-      - apply ForallMP_emptyMP.
-    Qed.
+(*     Lemma SvmInvs_init: *)
+(*       SvmInvs (initsOf impl0). *)
+(*     Proof. *)
+(*       repeat constructor. *)
+(*       - hnf; intros. *)
+(*         elim H. *)
+(*       - apply ForallMP_emptyMP. *)
+(*     Qed. *)
     
-  End Facts.
+(*   End Facts. *)
   
-End Sim.
+(* End Sim. *)
 
