src/IList.v
@@ -1,0 +1,205 @@
+(** Borrowed from the Fiat project
+ * (merged with VectorFacts.v in the same directory):
+ * https://github.mit.edu/plv/fiat/blob/master/src/Common/ilist.v
+ *)
+
+Generalizable All Variables.
+Set Implicit Arguments.
+
+Require Import Coq.Lists.List
+        Coq.Strings.String
+        Coq.Arith.Arith.
+Require Vector.
+
+Import Vectors.VectorDef.VectorNotations.
+
+Definition Vector_caseS'
+           {A'} (Q : nat -> Type)
+           (P : forall {n} (v : Vector.t A' (S n)), Q n -> Type)
+           (H : forall h {n} t q, @P n (h :: t) q) {n} (v: Vector.t A' (S n))
+           (q : Q n)
+  : P v q.
+Proof.
+  specialize (fun h t => H h _ t q).
+  change n with (pred (S n)) in H, q |- *.
+  set (Sn := S n) in *.
+  pose (fun Sn (v : Vector.t A' Sn) (q : Q (pred Sn)) =>
+          match Sn return Vector.t A' Sn -> Q (pred Sn) -> Type with
+          | S n' => P n'
+          | 0 => fun _ _ => True
+          end v q) as P'.
+  change (match Sn return Type with
+          | 0 => True
+          | _ => P' Sn v q
+          end).
+  change (forall h (t : match Sn with
+                        | S n' => Vector.t A' n'
+                        | 0 => Vector.t A' Sn
+                        end),
+             P' Sn (match Sn return match Sn with
+                                    | S n' => Vector.t A' n'
+                                    | 0 => Vector.t A' Sn
+                                    end -> Vector.t A' Sn
+                    with
+                    | S _ => fun t => h :: t
+                    | 0 => fun t => t
+                    end t) q) in H.
+  clearbody P'; clear P.
+  clearbody Sn.
+  destruct v as [|h ? t].
+  { constructor. }
+  { apply H. }
+Defined.
+
+Section ilist.
+
+  (* Lists of elements whose types depend on an indexing set (CPDT's hlists).
+     These lists are a convenient way to implement finite maps
+     whose elements depend on their keys. The data structures used
+     by our ADT notations uses these to implement notation-friendly
+     method lookups.  *)
+
+  Context {A : Type}. (* The indexing type. *)
+  Context {B : A -> Type}. (* The type of indexed elements. *)
+
+  Record prim_prod A B : Type :=
+    { prim_fst : A;
+      prim_snd : B }.
+
+  Fixpoint ilist {n} (l : Vector.t A n) : Type :=
+    match l with
+    | [] => unit
+    | a :: l => @prim_prod (B a) (ilist l)
+    end.
+
+  Definition icons
+             (a : A)
+             {n}
+             {l : Vector.t A n}
+             (b : B a)
+             (il : ilist l)
+    : ilist (a :: l)
+    := {| prim_fst := b; prim_snd := il |}.
+
+  Definition inil : ilist [] := tt.
+
+  (* Get the car of an ilist. *)
+  Definition ilist_hd {n} {As : Vector.t A n} (il : ilist As) :
+    match As return ilist As -> Type with
+    | a :: As' => fun il => B a
+    | [] => fun _ => unit
+    end il :=
+    match As return
+          forall (il : ilist As),
+            match As return ilist As -> Type with
+            | a :: As' => fun il => B a
+            | [] => fun _ => unit
+            end il with
+    | a :: As => fun il => prim_fst il
+    | [] => fun il => tt
+    end il.
+
+  Definition ilist_hd' {n} {As : Vector.t A (S n)} (il : ilist As) :
+    B (Vector.hd As)
+    := Vector.caseS (fun n As => ilist As -> B (Vector.hd As))
+                    (fun a As m => ilist_hd) As il.
+
+  (* Get the cdr of an ilist. *)
+  Definition ilist_tl {n} {As : Vector.t A n} (il : ilist As) :
+    match As return ilist As -> Type with
+    | a :: As' => fun il => ilist As'
+    | [] => fun _ => unit
+    end il :=
+    match As return
+          forall (il : ilist As),
+            match As return ilist As -> Type with
+            | a :: As' => fun il => ilist As'
+            | [] => fun _ => unit
+            end il with
+    | a :: As => fun il => prim_snd il
+    | [] => fun il => tt
+    end il.
+
+  Definition ilist_tl'
+             {n} {As : Vector.t A (S n)} (il : ilist As)
+    : ilist (Vector.tl As) :=
+    Vector.caseS (fun n As => ilist As -> ilist (Vector.tl As))
+                 (fun a As m => ilist_tl) As il.
+
+  Infix "++" := Vector.append : vector_scope.
+
+  (* Appending ilists *)
+  Fixpoint ilist_app {n} {As : Vector.t A n}
+    : forall {n'} {As' : Vector.t A n'},  ilist As -> ilist As' -> ilist (As ++ As') :=
+    match As return
+          forall {n'} (As' : Vector.t A n'),
+            ilist As -> ilist As' -> ilist (As ++ As') with
+    | [] =>
+      fun n' As' il il' => il'
+    | a :: As'' =>
+      fun n' As' il il' =>
+        {| prim_fst := ilist_hd il;
+           prim_snd := ilist_app (ilist_tl il) il' |}
+    end.
+
+  (* Membership in an indexed list. *)
+
+  Inductive ilist_In {a : A} (b : B a)
+    : forall {n} {As : Vector.t A n} (il : ilist As), Prop :=
+  | In_hd : forall n' As' (il : ilist (n := n') As'),
+      ilist_In b (icons b il)
+  | In_tl : forall {n'} a' (b' : B a') As' (il : ilist (n := n') As'),
+      ilist_In b il ->
+      ilist_In b (icons b' il).
+
+  (* Looking up the ith value, returning None for indices not in the Vector.t *)
+
+  Fixpoint ith
+           {m : nat}
+           {As : Vector.t A m}
+           (il : ilist As)
+           (n : Fin.t m)
+    : B (Vector.nth As n) :=
+    match n in Fin.t m return
+          forall (As : Vector.t A m),
+            ilist As
+            -> B (Vector.nth As n) with
+    | Fin.F1 =>
+      fun As =>
+        Vector.caseS (fun n As => ilist As
+                                  -> B (Vector.nth As (@Fin.F1 n)))
+                     (fun h n t => ilist_hd) As
+    | Fin.FS n' =>
+      fun As =>
+        Vector_caseS' Fin.t
+                      (fun n As n' => ilist As
+                                      -> B (Vector.nth As (@Fin.FS n n')))
+                      (fun h n t m il => ith (ilist_tl il) m)
+                      As n'
+    end As il.
+
+  Lemma ilist_invert {n} (As : Vector.t A n) (il : ilist As) :
+    match As as As' return ilist As' -> Prop with
+    | a :: As' => fun il => exists b il', il = icons b il'
+    | [] => fun il => il = inil
+    end il.
+  Proof.
+    destruct As; destruct il; simpl; unfold icons; eauto.
+  Qed.
+
+  Lemma ilist_invert' {n} (As : Vector.t A n) (il : ilist As) :
+    match As as As' return ilist As' -> Type with
+    | a :: As' => fun il => sigT (fun b => sigT (fun il' => il = icons b il'))
+    | [] => fun il => il = inil
+    end il.
+  Proof.
+    destruct As; destruct il; unfold icons; eauto.
+  Qed.
+
+(* The [ith_induction] tactic is for working with lookups of bounded indices.
+     It first inducts on n, then destructs the index Vector.t [As] and eliminates
+     the contradictory cases, then finally destructs any indexed Vector.t in the
+     context with Bounds of [As]. *)
+
+End ilist.
+
