src/SemFacts.v
@@ -5,91 +5,35 @@ Require Import Omega.
 
 Set Implicit Arguments.
 
-Lemma addRules_indices:
-  forall rules sys,
-    oindsOf (addRules rules sys) = oindsOf sys.
-Proof.
-  reflexivity.
-Qed.
-
-Lemma addRules_OStates_inits:
-  forall rules sys,
-    initsOf (StateT:= OStates) (addRules rules sys) = initsOf sys.
-Proof.
-  reflexivity.
-Qed.
-
-Lemma addRules_TState_inits:
-  forall rules sys,
-    initsOf (StateT:= TState) (addRules rules sys) = initsOf sys.
-Proof.
-  reflexivity.
-Qed.
-
-Corollary addRules_behaviorOf:
-  forall sys rules hst,
-    behaviorOf (addRules rules sys) hst = behaviorOf sys hst.
-Proof.
-  induction hst; [reflexivity|].
-  simpl; rewrite IHhst; reflexivity.
-Qed.
-
-Lemma buildRawSys_oindsOf:
-  forall {SysT} `{IsSystem SysT} `{HasInit SysT OStates} (sys: SysT),
-    oindsOf sys = oindsOf (buildRawSys sys).
-Proof.
-  intros; unfold oindsOf, buildRawSys; simpl.
-  reflexivity.
-Qed.
-
-Lemma addRules_app:
-  forall sys rules1 rules2,
-    addRules (rules1 ++ rules2) sys =
-    addRules rules2 (addRules rules1 sys).
-Proof.
-  unfold addRules; simpl; intros.
-  rewrite app_assoc; reflexivity.
-Qed.
-
-Lemma addRulesSys_buildRawSys:
-  forall rules sys,
-    sys_rules (addRules rules (buildRawSys sys)) = rules.
-Proof.
-  reflexivity.
-Qed.
-
-Lemma mindsOf_merqsOf_DisjList:
-  forall {SysT} `{IsSystem SysT} (sys: SysT),
-    DisjList (mindsOf sys) (merqsOf sys).
+Lemma sys_minds_sys_merqs_DisjList:
+  forall sys, DisjList (sys_minds sys) (sys_merqs sys).
 Proof.
   intros.
   eapply DisjList_NoDup; [exact eq_nat_dec|].
   eapply NoDup_app_weakening_1.
   rewrite <-app_assoc.
-  apply msg_inds_valid.
+  apply sys_msg_inds_valid.
 Qed.
 
-Lemma merqsOf_merssOf_DisjList:
-  forall {SysT} `{IsSystem SysT} (sys: SysT),
-    DisjList (merqsOf sys) (merssOf sys).
+Lemma sys_merqs_sys_merss_DisjList:
+  forall sys, DisjList (sys_merqs sys) (sys_merss sys).
 Proof.
   intros.
   eapply DisjList_NoDup; [exact eq_nat_dec|].
   eapply NoDup_app_weakening_2.
-  apply msg_inds_valid.
+  apply sys_msg_inds_valid.
 Qed.
 
-Lemma mindsOf_merssOf_DisjList:
-  forall {SysT} `{IsSystem SysT} (sys: SysT),
-    DisjList (mindsOf sys) (merssOf sys).
+Lemma sys_minds_sys_merss_DisjList:
+  forall sys, DisjList (sys_minds sys) (sys_merss sys).
 Proof.
   intros.
   eapply DisjList_NoDup; [exact eq_nat_dec|].
-  pose proof (msg_inds_valid sys).
-  rewrite app_assoc in H0.
-  apply NoDup_app_comm in H0.
-  rewrite app_assoc in H0.
-  apply NoDup_app_weakening_1 in H0.
+  pose proof (sys_msg_inds_valid sys).
+  rewrite app_assoc in H.
+  apply NoDup_app_comm in H.
+  rewrite app_assoc in H.
+  apply NoDup_app_weakening_1 in H.
   apply NoDup_app_comm; assumption.
 Qed.
 
@@ -126,62 +70,62 @@ Proof.
   inv H; rewrite H2; auto.
 Qed.
 
-Lemma ValidMsgsIn_mindsOf:
-  forall {MsgT SysT} `{HasMsg MsgT} `{IsSystem SysT}
-         (sys1: SysT) (eins: list (Id MsgT)),
+Lemma ValidMsgsIn_sys_minds:
+  forall {MsgT} `{HasMsg MsgT}
+         (sys1: System) (eins: list (Id MsgT)),
     ValidMsgsIn sys1 eins ->
     forall sys2,
-      mindsOf sys1 = mindsOf sys2 ->
+      sys_minds sys1 = sys_minds sys2 ->
       ValidMsgsIn sys2 eins.
 Proof.
   unfold ValidMsgsIn; intros.
   dest; split; auto.
-  rewrite <-H2; assumption.
+  rewrite <-H1; assumption.
 Qed.
 
-Lemma ValidMsgsOut_mindsOf_merssOf:
-  forall {MsgT SysT} `{HasMsg MsgT} `{IsSystem SysT}
-         (sys1: SysT) (eouts: list (Id MsgT)),
+Lemma ValidMsgsOut_sys_minds_sys_merss:
+  forall {MsgT} `{HasMsg MsgT} 
+         (sys1: System) (eouts: list (Id MsgT)),
     ValidMsgsOut sys1 eouts ->
     forall sys2,
-      mindsOf sys1 = mindsOf sys2 ->
-      merssOf sys1 = merssOf sys2 ->
+      sys_minds sys1 = sys_minds sys2 ->
+      sys_merss sys1 = sys_merss sys2 ->
       ValidMsgsOut sys2 eouts.
 Proof.
   unfold ValidMsgsOut; intros.
   dest; split; auto.
-  rewrite <-H2, <-H3; assumption.
+  rewrite <-H1, <-H2; assumption.
 Qed.
 
-Lemma ValidMsgsExtIn_merqsOf:
-  forall {MsgT SysT} `{HasMsg MsgT} `{IsSystem SysT}
-         (sys1: SysT) (eins: list (Id MsgT)),
+Lemma ValidMsgsExtIn_sys_merqs:
+  forall {MsgT} `{HasMsg MsgT} 
+         (sys1: System) (eins: list (Id MsgT)),
     ValidMsgsExtIn sys1 eins ->
     forall sys2,
-      merqsOf sys1 = merqsOf sys2 ->
+      sys_merqs sys1 = sys_merqs sys2 ->
       ValidMsgsExtIn sys2 eins.
 Proof.
   unfold ValidMsgsExtIn; intros.
   dest; split; auto.
-  rewrite <-H2; assumption.
+  rewrite <-H1; assumption.
 Qed.
   
-Lemma ValidMsgsExtOut_merssOf:
-  forall {MsgT SysT} `{HasMsg MsgT} `{IsSystem SysT}
-         (sys1: SysT) (eouts: list (Id MsgT)),
+Lemma ValidMsgsExtOut_sys_merss:
+  forall {MsgT} `{HasMsg MsgT} 
+         (sys1: System) (eouts: list (Id MsgT)),
     ValidMsgsExtOut sys1 eouts ->
     forall sys2,
-      merssOf sys1 = merssOf sys2 ->
+      sys_merss sys1 = sys_merss sys2 ->
       ValidMsgsExtOut sys2 eouts.
 Proof.
   unfold ValidMsgsExtOut; intros.
   dest; split; auto.
-  rewrite <-H2; assumption.
+  rewrite <-H1; assumption.
 Qed.
 
 Lemma step_t_tid_next:
-  forall sys st1 orule ins outs ts st2,
-    step_t sys st1 (RlblInt orule ins outs) st2 ->
+  forall sys st1 oidx ridx ins outs ts st2,
+    step_t sys st1 (RlblInt oidx ridx ins outs) st2 ->
     outs <> nil ->
     Forall (fun tmsg => tmsg_info tmsg = None) (valsOf ins) ->
     Forall (fun tmsg => match tmsg_info tmsg with
@@ -201,11 +145,11 @@ Proof.
   - inv H2; simpl in H3; auto.
 Qed.
 
-Lemma extRssOf_In_merssOf_FirstMP:
-  forall {SysT} `{IsSystem SysT} (sys: SysT) msgs1 msgs2,
+Lemma extRssOf_In_sys_merss_FirstMP:
+  forall (sys: System) msgs1 msgs2,
     extRssOf sys msgs1 = extRssOf sys msgs2 ->
     forall mout,
-      In (idOf mout) (merssOf sys) ->
+      In (idOf mout) (sys_merss sys) ->
       FirstMP msgs1 (idOf mout) (valOf mout) ->
       FirstMP msgs2 (idOf mout) (valOf mout).
 Proof.
@@ -213,23 +157,23 @@ Proof.
   eapply qsOf_In_FirstMP; eauto.
 Qed.
 
-Corollary extRssOf_SubList_merssOf_FirstMP:
-  forall {SysT} `{IsSystem SysT} (sys: SysT) msgs1 msgs2,
+Corollary extRssOf_SubList_sys_merss_FirstMP:
+  forall (sys: System) msgs1 msgs2,
     extRssOf sys msgs1 = extRssOf sys msgs2 ->
     forall mouts,
-      SubList (idsOf mouts) (merssOf sys) ->
+      SubList (idsOf mouts) (sys_merss sys) ->
       Forall (FirstMPI msgs1) mouts ->
       Forall (FirstMPI msgs2) mouts.
 Proof.
   induction mouts; simpl; intros; [constructor|].
-  apply SubList_cons_inv in H1; dest.
-  inv H2; constructor; auto.
+  apply SubList_cons_inv in H0; dest.
+  inv H1; constructor; auto.
   unfold FirstMPI in *.
-  eauto using extRssOf_In_merssOf_FirstMP.
+  eauto using extRssOf_In_sys_merss_FirstMP.
 Qed.
 
-Corollary extRssOf_ValidMsgsExtOut_merssOf_FirstMP:
-  forall {SysT} `{IsSystem SysT} (sys: SysT) msgs1 msgs2,
+Corollary extRssOf_ValidMsgsExtOut_sys_merss_FirstMP:
+  forall (sys: System) msgs1 msgs2,
     extRssOf sys msgs1 = extRssOf sys msgs2 ->
     forall mouts,
       ValidMsgsExtOut sys mouts ->
@@ -237,8 +181,8 @@ Corollary extRssOf_ValidMsgsExtOut_merssOf_FirstMP:
       Forall (FirstMPI msgs2) mouts.
 Proof.
   intros.
-  destruct H1.
-  eauto using extRssOf_SubList_merssOf_FirstMP.
+  destruct H0.
+  eauto using extRssOf_SubList_sys_merss_FirstMP.
 Qed.
 
 Lemma steps_wfHistory:
@@ -249,6 +193,7 @@ Proof.
   induction 1; simpl; intros; [constructor|].
   constructor; auto.
   clear H; inv H0; red; auto 7.
+  do 2 eexists; eauto 9.
 Qed.
 
 Theorem step_t_sound:
@@ -262,11 +207,11 @@ Theorem step_t_sound:
         TStateRel ntst nst.
 Proof.
   (* TODO: soundness of [step_t] *)
-Admitted.
+Abort.
 
 Lemma steps_split:
-  forall {SysT StateT LabelT} `{IsSystem SysT}
-         (step: Step SysT StateT LabelT) sys st1 st2 ll,
+  forall {StateT LabelT} 
+         (step: Step StateT LabelT) sys st1 st2 ll,
     steps step sys st1 ll st2 ->
     forall ll1 ll2,
       ll = ll2 ++ ll1 ->
@@ -274,18 +219,18 @@ Lemma steps_split:
         steps step sys st1 ll1 sti /\
         steps step sys sti ll2 st2.
 Proof.
-  induction 2; simpl; intros.
-  - apply eq_sym, app_eq_nil in H0; dest; subst.
+  induction 1; simpl; intros.
+  - apply eq_sym, app_eq_nil in H; dest; subst.
     eexists; split; econstructor.
   - destruct ll2.
-    + simpl in H2; subst.
+    + simpl in H1; subst.
       specialize (IHsteps ll nil eq_refl).
       destruct IHsteps as [tsi [? ?]].
-      inv H3.
+      inv H2.
       eexists; split.
       * econstructor; eauto.
       * econstructor.
-    + simpl in H2; inv H2.
+    + simpl in H1; inv H1.
       specialize (IHsteps _ _ eq_refl).
       destruct IHsteps as [sti [? ?]].
       eexists; split; eauto.
@@ -293,30 +238,28 @@ Proof.
 Qed.
 
 Lemma steps_append:
-  forall {SysT StateT LabelT} `{IsSystem SysT}
-         (step: Step SysT StateT LabelT) sys st1 ll1 st2,
+  forall {StateT LabelT} 
+         (step: Step StateT LabelT) sys st1 ll1 st2,
     steps step sys st1 ll1 st2 ->
     forall ll2 st3,
       steps step sys st2 ll2 st3 ->
       steps step sys st1 (ll2 ++ ll1) st3.
 Proof.
-  induction 3; simpl; intros; [auto|].
+  induction 2; simpl; intros; [auto|].
   econstructor; eauto.
 Qed.
 
 Lemma reachable_init:
-  forall {SysT StateT LabelT}
-         `{IsSystem SysT} `{HasInit SysT StateT} `{HasLabel LabelT}
-         (step: Step SysT StateT LabelT) sys,
+  forall {StateT LabelT} `{HasInit System StateT} `{HasLabel LabelT}
+         (step: Step StateT LabelT) sys,
     Reachable (steps step) sys (initsOf sys).
 Proof.
   eexists; econstructor.
 Qed.
 
 Lemma reachable_steps:
-  forall {SysT StateT LabelT}
-         `{IsSystem SysT} `{HasInit SysT StateT} `{HasLabel LabelT}
-         (step: Step SysT StateT LabelT) sys st1,
+  forall {StateT LabelT} `{HasInit System StateT} `{HasLabel LabelT}
+         (step: Step StateT LabelT) sys st1,
     Reachable (steps step) sys st1 ->
     forall ll st2,
       steps step sys st1 ll st2 ->
@@ -327,44 +270,32 @@ Proof.
 Qed.
   
 Lemma behaviorOf_app:
-  forall (sys: System)
-         {LabelT} `{HasLabel LabelT} (hst1 hst2: list LabelT),
-    behaviorOf sys (hst1 ++ hst2) =
-    behaviorOf sys hst1 ++ behaviorOf sys hst2.
+  forall {LabelT} `{HasLabel LabelT} (hst1 hst2: list LabelT),
+    behaviorOf (hst1 ++ hst2) =
+    behaviorOf hst1 ++ behaviorOf hst2.
 Proof.
   induction hst1; simpl; intros; auto.
   rewrite IHhst1.
   destruct (getLabel a); reflexivity.
 Qed.
 
-Lemma behaviorOf_preserved:
-  forall {SysT1 SysT2} `{IsSystem SysT1} `{IsSystem SysT2}
-         (impl1: SysT1) (impl2: SysT2),
-    oindsOf impl1 = oindsOf impl2 ->
-    forall {LabelT} `{HasLabel LabelT} (hst: list LabelT),
-      behaviorOf impl1 hst = behaviorOf impl2 hst.
-Proof.
-  induction hst; simpl; intros; [reflexivity|].
-  rewrite IHhst; reflexivity.
-Qed.
-
 Theorem refines_refl:
-  forall {SysT StateT LabelT} `{IsSystem SysT} `{HasInit SysT StateT} `{HasLabel LabelT}
-         (ss: Steps SysT StateT LabelT) sys, ss # ss |-- sys ⊑ sys.
+  forall {StateT LabelT} `{HasInit System StateT} `{HasLabel LabelT}
+         (ss: Steps StateT LabelT) sys, ss # ss |-- sys ⊑ sys.
 Proof.
   unfold Refines; intros.
   assumption.
 Qed.
 
 Theorem refines_trans:
-  forall {SysT StateT LabelT} `{IsSystem SysT} `{HasInit SysT StateT} `{HasLabel LabelT}
-         (ss1 ss2 ss3: Steps SysT StateT LabelT) s1 s2 s3,
+  forall {StateT LabelT} `{HasInit System StateT} `{HasLabel LabelT}
+         (ss1 ss2 ss3: Steps StateT LabelT) s1 s2 s3,
     ss1 # ss2 |-- s1 ⊑ s2 ->
     ss2 # ss3 |-- s2 ⊑ s3 ->
     ss1 # ss3 |-- s1 ⊑ s3.
 Proof.
   unfold Refines; intros.
-  specialize (H3 _ (H2 _ H4)).
+  specialize (H2 _ (H1 _ H3)).
   assumption.
 Qed.
 
